Add proof for total correcness for procedures

Hoare_Triple.v
@@ -14,13 +14,17 @@ Definition precondition : Type := sigma -> Prop.
 
 Definition empty_precondition : precondition := (fun _ => False).
 
-(** Definition of Postcondtion **)
+(** Definition of Postcondition **)
 
 Definition postcondition : Type := sigma -> sigma -> Prop.
 
 Definition empty_postcondition :  postcondition := (fun _ _ => True).
 
-(** Defintion of functional correcness i.e Hoare Triples **)
+(** ------------------------------ **)
+(** Partial correcness             **)
+(** ------------------------------ **)
+
+(** Definition of functional correcness i.e Hoare Triples **)
 
 Definition hoare_triple (P : precondition) (Q: postcondition) (c : com) (ps : Psi.psi) : Prop :=
   forall s s',  P s -> ceval c s ps s' -> Q s' s.
@@ -92,7 +96,6 @@ Definition get_post (an:clause) :=
           post.
 
 (** Defintion of contract environments : *)
-(*     a map from procedure name to clauses **)
 
 Module Phi.
 
@@ -107,19 +110,19 @@ End Phi.
 Definition i_hoare_triple (n: nat)
   (P: precondition) (Q: postcondition)
   (c : com) (ps : Psi.psi) : Prop :=
-  forall s s',  P s -> ceval c s (k_inliner_ps n ps) s'  -> Q s' s.
+  forall s s',  P s -> ceval c s (Inline1.k_inliner_ps n ps) s'  -> Q s' s.
 
 Lemma i_hoare_triple_hoare_triple :
   forall P Q p ps,
-  hoare_triple P Q p ps <-> forall n, i_hoare_triple n P Q p ps.
+  hoare_triple P Q (CCall p) ps <-> forall n, i_hoare_triple n P Q (CCall p) ps.
 Proof.
 unfold hoare_triple, i_hoare_triple;split;intros H.
 * intros n s s' Pre Heval.
   eapply H.
   apply Pre.
-  eapply (n_inline_ps_ceval _ _ _ _ _ Heval).
+  eapply (Inline1.n_inline_ps_ceval _ _ _ _ _ Heval).
 * intros s s' HPre Heval.
-  apply ceval_n_inline_ps in Heval.
+  apply Inline1.ceval_n_inline_ps in Heval.
   destruct Heval.
   eapply H.
   + apply HPre.
@@ -155,7 +158,7 @@ induction n.
   eapply H.
   + apply IHn.
   + apply HPre.
-  + apply n_inline_ps_inline in Heval.
+  + apply Inline1.n_inline_ps_inline in Heval.
     apply Heval.
 Qed.
 
@@ -184,6 +187,10 @@ apply recursion_hoare_triple with cl.
 assumption.
 apply H.
 Qed.
+
+(** ------------------------------ **)
+(** Total correcness               **)
+(** ------------------------------ **)
 
 (** Definition of total correcness **)
 
@@ -290,7 +297,7 @@ Lemma while_total :
   forall (inv: assertion) (var: variant) b c ps l,
     total (fun s1 => inv (s1 :: l) /\ beval s1 b = true)
           (fun s2 s1 => inv (s2 :: l) /\ var s2 < var s1) c ps ->
-    (forall s1, inv (s1 :: l) -> 1 <= var s1) ->
+    (forall s1, inv (s1 :: l) -> 0 <= var s1) ->
     total (fun s => inv (s :: l))
                 (fun s' _ => inv (s' :: l) /\ beval s'  b = false)
                 (CWhile b c inv var) ps.
@@ -316,22 +323,119 @@ Proof.
       specialize (Hvariant x H0).
       assert (H2: v x <= v st - v st).
       { apply H1. reflexivity. }
-      replace (v st - v st) with 0 in H2.
+      replace (v st - v st) with 0 in H2;[| rewrite Proc.sub_diag;auto].
+      assert (HPrex: P(x :: l) /\ beval x b = true). { split;repeat assumption. }
+      specialize (Hhoare x HPrex).
+      destruct Hhoare.
       Lia.lia.
-      Search( _ - _ = 0).
-      rewrite Proc.sub_diag.
-      reflexivity.
     + apply E_WhileFalse.
       assumption.
 Qed.
 
+(** Total correcness for a com with procedure context **)
 
-(* Lemma func_total : *)
-(*   forall (inv: assertion) (var: variant) b c ps l, *)
-(*     total (fun s1 => inv (s1 :: l) /\ beval s1 b = true) *)
-(*           (fun s2 s1 => inv (s2 :: l) /\ var s2 < var s1) c ps -> *)
-(*     (forall s1, inv (s1 :: l) -> 1 <= var s1) -> *)
-(*     total (fun s => inv (s :: l)) *)
-(*                 (fun s' _ => inv (s' :: l) /\ beval s'  b = false) *)
-(*                 (CWhile b c inv var) ps. *)
-(* Proof. *)
+Definition total_ctx (cl : Phi.phi) (ps: Psi.psi)
+  (P: precondition) (Q: postcondition)  (c: com) :=
+  (forall p, total (get_pre (cl p)) (get_post (cl p)) (CCall p) ps) -> total P Q c ps.
+
+(** Total correcness for a procedure with procedure context **)
+
+Definition total_proc_ctx (var: variant) (cl : Phi.phi) (ps_init :Psi.psi) :=
+  forall v p ps,
+    (forall p, total (fun s => get_pre (cl p) s /\ var s + 1 = v)
+            (get_post (cl p))
+          (CCall p) ps) ->
+    total (fun s => get_pre (cl p) s /\ var s = v) (get_post (cl p))
+      (ps_init p) ps.
+
+(** Defintion of a Hoare Triple with inliner **)
+
+Definition i_total (n: nat)
+  (P: precondition) (Q: postcondition)
+  (c : com) (ps : Psi.psi) : Prop :=
+  forall s ,  P s -> (exists s', ceval (Inline2.k_inliner n c ps) s ps s' /\ Q s' s).
+
+Definition total_proc_ctx_n (n : nat) (var: variant) (cl : Phi.phi) (ps :Psi.psi) :=
+  forall v p,
+    (forall p, total (fun s => get_pre (cl p) s /\ var s + 1 = v - n )
+            (get_post (cl p))
+          (CCall p) ps) ->
+    i_total n (fun s => get_pre (cl p) s /\ var s = v) (get_post (cl p))
+      (CCall p) ps.
+
+Lemma total_proc_ctx_total_proc_ctx_n (var: variant) (cl : Phi.phi) (ps :Psi.psi) :
+  total_proc_ctx var cl ps -> forall n, total_proc_ctx_n n var cl ps.
+Proof.
+  intros H.
+  induction n;intros v p H0 s HPre.
+  - rewrite Proc.sub_0_r in H0.
+    specialize (H v p ps H0 s HPre).
+    destruct H.
+    destruct H.
+    exists x.
+    split;[|auto].
+    apply E_Call.
+    apply H.
+  -
+    assert (Hi: forall p,
+               total (fun s : sigma => get_pre (cl p) s /\ var s + 1 = v )
+                 (get_post (cl p)) (CCall p) ps).
+    { intros p0 s0 HP.
+      specialize (IHn (v - 1) p0).
+      replace (v - 1 - n ) with (v - S n ) in IHn by Lia.lia.
+      destruct HP.
+      apply Proc.add_sub_eq_r in H2.
+      symmetry in H2.
+      assert (HP : get_pre (cl p0) s0 /\ var s0 = v - 1) by auto.
+      specialize (IHn H0 s0 HP).
+      destruct IHn.
+      exists x.
+      destruct H3.
+      apply Inline2.n_inline_ceval_ceval in H3.
+      split; [apply H3 |  apply H4] .
+    }
+    specialize (H v p ps Hi s HPre).
+    destruct H.
+    exists x.
+    split;[|apply H].
+    apply Inline2.ceval_n_inline_ceval.
+    apply E_Call.
+    apply H.
+Qed.
+
+Lemma total_recursive_proc var ps cl:
+    (forall n, total_proc_ctx_n n var cl ps) ->
+   (forall p, total (get_pre (cl p)) (get_post (cl p)) (CCall p) ps).
+Proof.
+  intros.
+  intros s Hpre.
+  assert (H1:  (forall p : Proc.t,
+                   total (fun s0 : sigma => get_pre (cl p) s0 /\ var s0 + 1 = var s - var s)
+                     (get_post (cl p)) (CCall p) ps)).
+  { intros.
+    intros s' HP.
+    Lia.lia.}.
+  assert (HP:  get_pre (cl p) s /\ var s = var s);auto.
+  specialize (H (var s) (var s) p H1 s HP).
+  destruct H.
+  exists x.
+  destruct H.
+  split;[|auto].
+  apply Inline2.n_inline_ceval_ceval in H.
+  eauto.
+Qed.
+
+(** Modular Hoare Triple Verification **)
+
+Theorem recursion_total :
+  forall P Q p var ps cl,
+    total_proc_ctx var cl ps  ->
+    total_ctx cl ps P Q p ->
+    total P Q p ps.
+Proof.
+intros.
+apply H0.
+eapply total_recursive_proc.
+apply total_proc_ctx_total_proc_ctx_n.
+apply H.
+Qed.
