Inliner.v
@@ -16,219 +16,221 @@ Fixpoint inliner c inline :=
   | CWhile b p inv var => CWhile b (inliner p inline) inv var
   | CCall f => inline f
   | _ => c
-end.
+  end.
 
-(** Function for recursive procedure inlining in Com **)
+Module Inline1.
 
-Fixpoint k_inliner n c (ps : Psi.psi) :=
-  match n with
-  | 0 => CWhile BTrue CSkip (fun _ => True) (fun _ => 0)
-  | S n' => inliner c (fun f => k_inliner n' (ps f) ps)
-end.
+  (** Function for recursive procedure inlining in Com **)
 
-(** Function for procedure inlining in Psi.psi **)
+  Fixpoint k_inliner n c (ps : Psi.psi) :=
+    match n with
+    | 0 => CWhile BTrue CSkip (fun _ => True) (fun _ => 0)
+    | S n' => inliner c (fun f => k_inliner n' (ps f) ps)
+    end.
 
-Definition k_inliner_ps n ps := fun p => k_inliner n (ps p) ps.
+  (** Function for procedure inlining in Psi.psi **)
 
-(** Some fact about the inlining **)
+  Definition k_inliner_ps n ps := fun p => k_inliner n (ps p) ps.
 
-Lemma inline_cskip n ps : k_inliner (S n) CSkip ps = CSkip.
-Proof.
- reflexivity.
-Qed.
+  (** Some fact about the inlining **)
 
-Lemma inline_cass n ps x a1: k_inliner (S n) (CAss x a1) ps = (CAss x a1).
-Proof.
- reflexivity.
-Qed.
+  Lemma inline_cskip n ps : k_inliner (S n) CSkip ps = CSkip.
+  Proof.
+    reflexivity.
+  Qed.
 
-Lemma inline_cassr n ps x a1: k_inliner (S n) (CAssr x a1) ps = (CAssr x a1).
-Proof.
- reflexivity.
-Qed.
+  Lemma inline_cass n ps x a1: k_inliner (S n) (CAss x a1) ps = (CAss x a1).
+  Proof.
+    reflexivity.
+  Qed.
 
-Lemma inline_cassert n ps b: k_inliner (S n) (CAssert b) ps = (CAssert b).
-Proof.
- reflexivity.
-Qed.
+  Lemma inline_cassr n ps x a1: k_inliner (S n) (CAssr x a1) ps = (CAssr x a1).
+  Proof.
+    reflexivity.
+  Qed.
 
-Lemma inline_cseq n ps p1 p2: k_inliner (S n) (CSeq p1 p2) ps =
-                              CSeq (k_inliner (S n) p1 ps) (k_inliner (S n) p2 ps).
-Proof.
- reflexivity.
-Qed.
+  Lemma inline_cassert n ps b: k_inliner (S n) (CAssert b) ps = (CAssert b).
+  Proof.
+    reflexivity.
+  Qed.
 
-Lemma inline_cif n ps b p1 p2: k_inliner (S n) (CIf b p1 p2) ps =
-                               CIf b (k_inliner (S n)  p1 ps) (k_inliner (S n) p2 ps).
-Proof.
- reflexivity.
-Qed.
+  Lemma inline_cseq n ps p1 p2: k_inliner (S n) (CSeq p1 p2) ps =
+                                  CSeq (k_inliner (S n) p1 ps) (k_inliner (S n) p2 ps).
+  Proof.
+    reflexivity.
+  Qed.
 
-Lemma inline_cwhile n ps p b inv var: k_inliner (S n) (CWhile b p inv var) ps =
-                                  CWhile b (k_inliner (S n) p ps) inv var.
-Proof.
- reflexivity.
-Qed.
+  Lemma inline_cif n ps b p1 p2: k_inliner (S n) (CIf b p1 p2) ps =
+                                   CIf b (k_inliner (S n)  p1 ps) (k_inliner (S n) p2 ps).
+  Proof.
+    reflexivity.
+  Qed.
 
-Lemma inline_ccall n f ps :
-   k_inliner (S n) (CCall f) ps = k_inliner n (ps f) ps.
-Proof.
- reflexivity.
-Qed.
+  Lemma inline_cwhile n ps p b inv var: k_inliner (S n) (CWhile b p inv var) ps =
+                                          CWhile b (k_inliner (S n) p ps) inv var.
+  Proof.
+    reflexivity.
+  Qed.
 
-(* ceval is inlining insensitive on command *)
+  Lemma inline_ccall n f ps :
+    k_inliner (S n) (CCall f) ps = k_inliner n (ps f) ps.
+  Proof.
+    reflexivity.
+  Qed.
 
-Lemma ceval_inline p s ps s':
-  ceval p s ps s' -> ceval (inliner p ps) s ps s'.
-Proof.
-intros.
-induction H.
-  + apply E_Skip.
-  + apply E_Ass.
-    all: try now auto.
-  + apply E_Assr.
-    all: try now auto.
-  + apply E_Assert.
-  + simpl. apply E_IfTrue; [now auto | now auto].
-  + simpl. apply E_IfFalse; [now auto | now auto].
-  + simpl. eapply E_Seq.
+  (* ceval is inlining insensitive on command *)
+
+  Lemma ceval_inline p s ps s':
+    ceval p s ps s' -> ceval (inliner p ps) s ps s'.
+  Proof.
+    intros.
+    induction H.
+    + apply E_Skip.
+    + apply E_Ass.
+      all: try now auto.
+    + apply E_Assr.
+      all: try now auto.
+    + apply E_Assert.
+    + simpl. apply E_IfTrue; [now auto | now auto].
+    + simpl. apply E_IfFalse; [now auto | now auto].
+    + simpl. eapply E_Seq.
     - apply IHceval1.
     - apply IHceval2.
-  + apply E_WhileFalse; now auto.
-  + simpl. eapply E_WhileTrue; [now auto | | ].
+      + apply E_WhileFalse; now auto.
+      + simpl. eapply E_WhileTrue; [now auto | | ].
     - apply IHceval1.
     - apply IHceval2.
-  + simpl. assumption.
-Qed.
+      + simpl. assumption.
+  Qed.
 
-Lemma inline_ceval p s ps s':
-  ceval (inliner p ps) s ps s' -> ceval p s ps s'.
-Proof.
-intros.
-generalize dependent s.
-generalize dependent s'.
-generalize dependent ps.
-induction p;intros.
-  + inversion H;subst.
-    apply E_Skip.
-  + inversion H;subst.
-    apply E_Ass. all: try now auto.
-  + inversion H;subst.
-    apply E_Assr. all: try now auto.
-  + inversion H;subst.
-    apply E_Assert.
-  + inversion H;subst.
-    eapply E_Seq.
-    * apply IHp1. apply H2.
-    * apply IHp2. apply H6.
-  + inversion H;subst.
-    * eapply E_IfTrue.
-      assumption.
-      apply IHp1. apply H7.
-    * eapply E_IfFalse.
-      assumption.
-      apply IHp2. apply H7.
-   + remember (inliner (CWhile b p inv var) ps) as original_command eqn:Horig.
-     induction H; inversion Horig;subst.
-     * eapply E_WhileFalse.
-       assumption.
-     * eapply E_WhileTrue.
-       assumption.
-       apply IHp. apply H0.
-       apply IHceval2.
-       assumption.
-   + apply E_Call.
+  Lemma inline_ceval p s ps s':
+    ceval (inliner p ps) s ps s' -> ceval p s ps s'.
+  Proof.
+    intros.
+    generalize dependent s.
+    generalize dependent s'.
+    generalize dependent ps.
+    induction p;intros.
+    + inversion H;subst.
+      apply E_Skip.
+    + inversion H;subst.
+      apply E_Ass. all: try now auto.
+    + inversion H;subst.
+      apply E_Assr. all: try now auto.
+    + inversion H;subst.
+      apply E_Assert.
+    + inversion H;subst.
+      eapply E_Seq.
+      * apply IHp1. apply H2.
+      * apply IHp2. apply H6.
+    + inversion H;subst.
+      * eapply E_IfTrue.
+        assumption.
+        apply IHp1. apply H7.
+      * eapply E_IfFalse.
+        assumption.
+        apply IHp2. apply H7.
+    + remember (inliner (CWhile b p inv var) ps) as original_command eqn:Horig.
+      induction H; inversion Horig;subst.
+      * eapply E_WhileFalse.
+        assumption.
+      * eapply E_WhileTrue.
+        assumption.
+        apply IHp. apply H0.
+        apply IHceval2.
+        assumption.
+    + apply E_Call.
       simpl in H. assumption.
-Qed.
+  Qed.
 
-(* Inlining on Com "n+1" times is equivalent to inline on Psi.psi "n" times *)
+  (* Inlining on Com "n+1" times is equivalent to inline on Psi.psi "n" times *)
 
-Lemma n_inline_n_inline_ps n p s ps_init s' :
-   (forall ps, ceval (k_inliner (S n) p ps_init) s ps s') ->
-   ceval p s (k_inliner_ps n ps_init) s'.
-Proof.
-intros.
-specialize (H (k_inliner_ps n ps_init)).
-generalize dependent s.
-generalize dependent s'.
-induction p ;intros.
-* rewrite inline_cskip in H.
-  apply H.
-* rewrite inline_cass in H.
-  apply H.
-* rewrite inline_cassr in H.
-  apply H.
-* rewrite inline_cassert in H.
-  apply H.
-* rewrite inline_cseq in H.
-  inversion H;subst.
-  apply E_Seq with s'0.
-  + apply IHp1.
-    apply H2.
-  + apply IHp2.
-    apply H6.
-* rewrite inline_cif in H.
-  inversion H;subst.
-  + apply E_IfTrue.
+  Lemma n_inline_n_inline_ps n p s ps_init s' :
+    (forall ps, ceval (k_inliner (S n) p ps_init) s ps s') ->
+    ceval p s (k_inliner_ps n ps_init) s'.
+  Proof.
+    intros.
+    specialize (H (k_inliner_ps n ps_init)).
+    generalize dependent s.
+    generalize dependent s'.
+    induction p ;intros.
+    * rewrite inline_cskip in H.
+      apply H.
+    * rewrite inline_cass in H.
+      apply H.
+    * rewrite inline_cassr in H.
+      apply H.
+    * rewrite inline_cassert in H.
+      apply H.
+    * rewrite inline_cseq in H.
+      inversion H;subst.
+      apply E_Seq with s'0.
+    + apply IHp1.
+      apply H2.
+    + apply IHp2.
+      apply H6.
+      * rewrite inline_cif in H.
+        inversion H;subst.
+    + apply E_IfTrue.
     - assumption.
     - apply IHp1.
       apply H7.
-  + apply E_IfFalse.
+      + apply E_IfFalse.
     - assumption.
     - apply IHp2.
       apply H7.
-* remember (k_inliner (S n) (CWhile b p inv var) ps_init) as original_command eqn:Horig.
-  induction H;rewrite inline_cwhile in Horig; inversion Horig.
-  + inversion Horig;subst.
-     eapply E_WhileFalse.
-     assumption.
-  + inversion Horig;subst.
-    eapply E_WhileTrue.
+      * remember (k_inliner (S n) (CWhile b p inv var) ps_init) as original_command eqn:Horig.
+        induction H;rewrite inline_cwhile in Horig; inversion Horig.
+      + inversion Horig;subst.
+        eapply E_WhileFalse.
+        assumption.
+      + inversion Horig;subst.
+        eapply E_WhileTrue.
     - assumption.
     - apply IHp. apply H0.
     - apply IHceval2.
       assumption.
       rewrite <- inline_cwhile in Horig.
       apply Horig.
-* apply E_Call.
-  rewrite inline_ccall in H.
-  apply H.
-Qed.
+      * apply E_Call.
+        rewrite inline_ccall in H.
+        apply H.
+  Qed.
 
-Lemma inline_p_ps n p ps s s' ps1 ps2:
-ceval (k_inliner n p ps) s ps1 s' ->
-ceval (k_inliner n p ps) s ps2 s'.
-Proof.
-intros.
-generalize dependent s.
-generalize dependent s'.
-generalize dependent p.
-induction n.
-* intros.
-  apply ceval_inf_loop in H.
-  contradiction H.
-* induction p;intros.
-  + inversion H;subst.
-    apply E_Skip.
-  + inversion H;subst.
-    apply E_Ass.
-    all: try now auto.
-  + inversion H;subst.
-    apply E_Assr.
-    all: try now auto.
-  + inversion H;subst.
-    apply E_Assert.
-  + rewrite inline_cseq.
-    rewrite inline_cseq in H.
-    inversion H;subst.
-    apply E_Seq with s'0.
+  Lemma inline_p_ps n p ps s s' ps1 ps2:
+    ceval (k_inliner n p ps) s ps1 s' ->
+    ceval (k_inliner n p ps) s ps2 s'.
+  Proof.
+    intros.
+    generalize dependent s.
+    generalize dependent s'.
+    generalize dependent p.
+    induction n.
+    * intros.
+      apply ceval_inf_loop in H.
+      contradiction H.
+    * induction p;intros.
+    + inversion H;subst.
+      apply E_Skip.
+    + inversion H;subst.
+      apply E_Ass.
+      all: try now auto.
+    + inversion H;subst.
+      apply E_Assr.
+      all: try now auto.
+    + inversion H;subst.
+      apply E_Assert.
+    + rewrite inline_cseq.
+      rewrite inline_cseq in H.
+      inversion H;subst.
+      apply E_Seq with s'0.
     - apply IHp1.
       apply H2.
     - apply IHp2.
       apply H6.
-  + rewrite inline_cif.
-    rewrite inline_cif in H.
-    inversion H;subst.
+      + rewrite inline_cif.
+        rewrite inline_cif in H.
+        inversion H;subst.
     - apply E_IfTrue.
       assumption.
       apply IHp1.
@@ -237,8 +239,8 @@ induction n.
       assumption.
       apply IHp2.
       apply H7.
-  + remember (k_inliner (S n) (CWhile b p inv var) ps) as original_command eqn:Horig.
-    induction H;rewrite inline_cwhile in Horig; inversion Horig.
+      + remember (k_inliner (S n) (CWhile b p inv var) ps) as original_command eqn:Horig.
+        induction H;rewrite inline_cwhile in Horig; inversion Horig.
     - inversion Horig;subst.
       eapply E_WhileFalse.
       assumption.
@@ -251,86 +253,86 @@ induction n.
          assumption.
          rewrite <- inline_cwhile in Horig.
          apply Horig.
-  + apply IHn.
-    apply H.
-Qed.
+      + apply IHn.
+        apply H.
+  Qed.
 
-Lemma n_ps_inline_n_inline n p s ps_init s' :
-   ceval p s (k_inliner_ps n ps_init) s' ->
-   (forall ps, ceval (k_inliner (S n) p ps_init) s ps s').
-Proof.
-intros.
-generalize dependent s.
-generalize dependent s'.
-induction p;intros.
-* eapply inline_p_ps.
-  apply H.
-* eapply inline_p_ps.
-  apply H.
-* eapply inline_p_ps.
-  apply H.
-* eapply inline_p_ps.
-  apply H.
-* inversion H;subst.
-  apply E_Seq with s'0.
-  + apply IHp1.
-    apply H2.
-  + apply IHp2.
-    apply H6.
-* inversion H;subst.
-  + apply E_IfTrue.
+  Lemma n_ps_inline_n_inline n p s ps_init s' :
+    ceval p s (k_inliner_ps n ps_init) s' ->
+    (forall ps, ceval (k_inliner (S n) p ps_init) s ps s').
+  Proof.
+    intros.
+    generalize dependent s.
+    generalize dependent s'.
+    induction p;intros.
+    * eapply inline_p_ps.
+      apply H.
+    * eapply inline_p_ps.
+      apply H.
+    * eapply inline_p_ps.
+      apply H.
+    * eapply inline_p_ps.
+      apply H.
+    * inversion H;subst.
+      apply E_Seq with s'0.
+    + apply IHp1.
+      apply H2.
+    + apply IHp2.
+      apply H6.
+      * inversion H;subst.
+    + apply E_IfTrue.
     - assumption.
     - apply IHp1.
       assumption.
-  + apply E_IfFalse.
+      + apply E_IfFalse.
     - assumption.
     - apply IHp2.
       assumption.
-* remember (CWhile b p inv var) as original_command eqn:Horig.
-  induction H; try inversion Horig.
-  + inversion Horig;subst.
-     eapply E_WhileFalse.
-     assumption.
-  + inversion Horig;subst.
-    eapply E_WhileTrue.
+      * remember (CWhile b p inv var) as original_command eqn:Horig.
+        induction H; try inversion Horig.
+      + inversion Horig;subst.
+        eapply E_WhileFalse.
+        assumption.
+      + inversion Horig;subst.
+        eapply E_WhileTrue.
     - assumption.
     - apply IHp. apply H0.
     - apply IHceval2.
       assumption.
       reflexivity.
-* inversion H; subst.
-  rewrite inline_ccall.
-  eapply inline_p_ps.
-  apply H1.
-Qed.
+      * inversion H; subst.
+        rewrite inline_ccall.
+        eapply inline_p_ps.
+        apply H1.
+  Qed.
 
-(* ceval is "n" inlining insensitive on command *)
+  (* ceval is "n" inlining insensitive on command *)
 
-Lemma inline_n_ceval n p s ps_init s':
-  (forall ps, ceval (k_inliner n p ps_init) s ps s') -> ceval p s ps_init s'.
-Proof.
-intros.
-specialize (H ps_init).
-generalize dependent s.
-generalize dependent s'.
-generalize dependent p.
-generalize dependent ps_init.
-induction n.
-* intros.
-  apply ceval_inf_loop in H.
-  contradiction H.
-* induction p;intros.
-  + apply H.
-  + apply H.
-  + apply H.
-  + apply H.
-  + inversion H;subst.
-    apply E_Seq with s'0.
+  Lemma inline_n_ceval n p s ps_init s':
+    (forall ps, ceval (k_inliner n p ps_init) s ps s') -> ceval p s ps_init s'.
+  Proof.
+    intros.
+    specialize (H ps_init).
+    generalize dependent s.
+    generalize dependent s'.
+    generalize dependent p.
+    generalize dependent ps_init.
+    induction n.
+    * intros.
+      apply ceval_inf_loop in H.
+      contradiction H.
+    * induction p;intros.
+    + apply H.
+    + apply H.
+    + apply H.
+    + apply H.
+    + inversion H;subst.
+      apply E_Seq with s'0.
     - apply IHp1.
       apply H2.
     - apply IHp2.
       apply H6.
-  + inversion H;subst.
+      + inversion H;subst.
     - apply E_IfTrue.
       ** assumption.
       ** apply IHp1.
@@ -339,40 +341,40 @@ induction n.
       ** assumption.
       ** apply IHp2.
          assumption.
-   + remember (k_inliner (S n) (CWhile b p inv var) ps_init) as original_command eqn:Horig.
-     induction H; try inversion Horig.
-     - inversion Horig;subst.
-       eapply E_WhileFalse.
-       assumption.
-     - inversion Horig;subst.
-       eapply E_WhileTrue.
-       ** assumption.
-       ** apply IHp. apply H0.
-       ** apply IHceval2.
-          assumption.
-          reflexivity.
-  + apply inline_ceval.
-    apply IHn.
-    rewrite inline_ccall in H.
-    apply H.
-Qed.
+      + remember (k_inliner (S n) (CWhile b p inv var) ps_init) as original_command eqn:Horig.
+        induction H; try inversion Horig.
+    - inversion Horig;subst.
+      eapply E_WhileFalse.
+      assumption.
+    - inversion Horig;subst.
+      eapply E_WhileTrue.
+      ** assumption.
+      ** apply IHp. apply H0.
+      ** apply IHceval2.
+         assumption.
+         reflexivity.
+      + apply inline_ceval.
+        apply IHn.
+        rewrite inline_ccall in H.
+        apply H.
+  Qed.
 
-Lemma inline_ceval_S n p s ps_init  s' ps:
-  ceval (k_inliner n p ps_init) s ps s' ->
-  forall m, n <= m -> ceval (k_inliner m p ps_init) s ps s'.
-Proof.
-intros.
-generalize dependent s.
-generalize dependent s'.
-generalize dependent p.
-generalize dependent m.
-induction n.
-* intros.
-  apply ceval_inf_loop in H.
-  contradiction H.
-* destruct m as [| m].
-  + intros. inversion H0.
-  + induction p;intros.
+  Lemma inline_ceval_S n p s ps_init  s' ps:
+    ceval (k_inliner n p ps_init) s ps s' ->
+    forall m, n <= m -> ceval (k_inliner m p ps_init) s ps s'.
+  Proof.
+    intros.
+    generalize dependent s.
+    generalize dependent s'.
+    generalize dependent p.
+    generalize dependent m.
+    induction n.
+    * intros.
+      apply ceval_inf_loop in H.
+      contradiction H.
+    * destruct m as [| m].
+    + intros. inversion H0.
+    + induction p;intros.
     - apply H.
     - apply H.
     - apply H.
@@ -389,184 +391,287 @@ induction n.
       inversion H;subst.
       ** rewrite inline_cif.
          apply E_IfTrue.
-         ++ assumption.
-         ++ apply IHp1.
-            apply H8.
-      ** rewrite inline_cif.
-         apply E_IfFalse.
-         ++ assumption.
-         ++ apply IHp2.
-            apply H8.
-     - remember (k_inliner (S n) (CWhile b p inv var) ps_init) as original_command eqn:Horig.
-     induction H; try inversion Horig.
+      ++ assumption.
+      ++ apply IHp1.
+         apply H8.
+         ** rewrite inline_cif.
+            apply E_IfFalse.
+      ++ assumption.
+      ++ apply IHp2.
+         apply H8.
+    - remember (k_inliner (S n) (CWhile b p inv var) ps_init) as original_command eqn:Horig.
+      induction H; try inversion Horig.
       ** inversion Horig;subst.
          eapply E_WhileFalse.
          assumption.
       ** inversion Horig;subst.
          rewrite inline_cwhile.
          eapply E_WhileTrue.
-         ++ assumption.
-         ++ apply IHp. apply H1.
-         ++ apply IHceval2.
-            assumption.
-            assumption.
-            reflexivity.
-  - rewrite inline_ccall.
-    apply IHn.
-    now apply Nat.succ_le_mono.
-    apply H.
-Qed.
+      ++ assumption.
+      ++ apply IHp. apply H1.
+      ++ apply IHceval2.
+         assumption.
+         assumption.
+         reflexivity.
+    - rewrite inline_ccall.
+      apply IHn.
+      now apply Nat.succ_le_mono.
+      apply H.
+  Qed.
 
-Lemma ceval_inline_n p s ps_init s':
-  ceval p s ps_init s' -> exists n, forall ps, ceval (k_inliner n p ps_init) s ps s'.
-Proof.
-induction 1;intros.
-* exists 1.
-  apply E_Skip.
-* exists 1.
-  intros.
-  apply E_Ass.
-  all: try now auto.
-* exists 1.
-  intros.
-  apply E_Assr.
-  all: try now auto.
-* exists 1.
-  intros.
-  apply E_Assert.
-* destruct IHceval as [n IH].
-  exists n.
-  intros.
-  specialize (IH ps0).
-  destruct n.
-  - apply ceval_inf_loop in IH.
-    contradiction IH.
-  - rewrite inline_cif.
-    apply E_IfTrue.
-    assumption.
-    apply IH.
-* destruct IHceval as [n IH].
-  exists n.
-  intros.
-  specialize (IH ps0).
-  destruct n.
-  - apply ceval_inf_loop in IH.
-    contradiction IH.
-  - rewrite inline_cif.
-    apply E_IfFalse.
-    assumption.
-    apply IH.
-* destruct IHceval1 as [n1 IH1].
-  destruct IHceval2 as [n2 IH2].
-  exists (max n1 n2).
-  intros.
-  specialize (IH1 ps0).
-  specialize (IH2 ps0).
-  destruct n1 as [|n1].
-  + apply ceval_inf_loop in IH1.
-    contradiction IH1.
-  + destruct n2 as [|n2].
+  Lemma ceval_inline_n p s ps_init s':
+    ceval p s ps_init s' -> exists n, forall ps, ceval (k_inliner n p ps_init) s ps s'.
+  Proof.
+    induction 1;intros.
+    * exists 1.
+      apply E_Skip.
+    * exists 1.
+      intros.
+      apply E_Ass.
+      all: try now auto.
+    * exists 1.
+      intros.
+      apply E_Assr.
+      all: try now auto.
+    * exists 1.
+      intros.
+      apply E_Assert.
+    * destruct IHceval as [n IH].
+      exists n.
+      intros.
+      specialize (IH ps0).
+      destruct n.
+    - apply ceval_inf_loop in IH.
+      contradiction IH.
+    - rewrite inline_cif.
+      apply E_IfTrue.
+      assumption.
+      apply IH.
+      * destruct IHceval as [n IH].
+        exists n.
+        intros.
+        specialize (IH ps0).
+        destruct n.
+    - apply ceval_inf_loop in IH.
+      contradiction IH.
+    - rewrite inline_cif.
+      apply E_IfFalse.
+      assumption.
+      apply IH.
+      * destruct IHceval1 as [n1 IH1].
+        destruct IHceval2 as [n2 IH2].
+        exists (max n1 n2).
+        intros.
+        specialize (IH1 ps0).
+        specialize (IH2 ps0).
+        destruct n1 as [|n1].
+      + apply ceval_inf_loop in IH1.
+        contradiction IH1.
+      + destruct n2 as [|n2].
     - apply ceval_inf_loop in IH2.
       contradiction IH2.
     - destruct (Nat.max_dec (S n1) (S n2)).
       ** rewrite e.
          rewrite inline_cseq.
          apply E_Seq with s'. 
-         ++ apply inline_ceval_S with (S n1); [now auto | reflexivity].
-         ++ apply inline_ceval_S with (S n2); [now auto | now apply PeanoNat.Nat.max_l_iff].
-      ** rewrite e.
-         rewrite inline_cseq.
-         apply E_Seq with s'. 
-         ++ apply inline_ceval_S with (S n1); [now auto | now apply PeanoNat.Nat.max_r_iff].
-         ++ apply inline_ceval_S with (S n2); [now auto | reflexivity].
-* exists 1. intros. rewrite inline_cwhile. apply E_WhileFalse; now auto.
-* destruct IHceval1 as [n1 IH1].
-  destruct IHceval2 as [n2 IH2].
-  exists (max n1 n2).
-  intros.
-  specialize (IH1 ps0).
-  specialize (IH2 ps0).
-  destruct n1 as [|n1].
-  + apply ceval_inf_loop in IH1.
-    contradiction IH1.
-  + destruct n2 as [|n2].
+      ++ apply inline_ceval_S with (S n1); [now auto | reflexivity].
+      ++ apply inline_ceval_S with (S n2); [now auto | now apply PeanoNat.Nat.max_l_iff].
+         ** rewrite e.
+            rewrite inline_cseq.
+            apply E_Seq with s'. 
+      ++ apply inline_ceval_S with (S n1); [now auto | now apply PeanoNat.Nat.max_r_iff].
+      ++ apply inline_ceval_S with (S n2); [now auto | reflexivity].
+      * exists 1. intros. rewrite inline_cwhile. apply E_WhileFalse; now auto.
+      * destruct IHceval1 as [n1 IH1].
+        destruct IHceval2 as [n2 IH2].
+        exists (max n1 n2).
+        intros.
+        specialize (IH1 ps0).
+        specialize (IH2 ps0).
+        destruct n1 as [|n1].
+      + apply ceval_inf_loop in IH1.
+        contradiction IH1.
+      + destruct n2 as [|n2].
     - apply ceval_inf_loop in IH2.
       contradiction IH2.
     - destruct (Nat.max_dec (S n1) (S n2)).
       ** rewrite e.
          rewrite inline_cwhile.
          apply E_WhileTrue with s'; [now auto | | ].
-         ++ apply inline_ceval_S with (S n1); [now auto | reflexivity].
-         ++ rewrite <- inline_cwhile.
-            apply inline_ceval_S with (S n2); [now auto | now apply PeanoNat.Nat.max_l_iff].
-      ** rewrite e.
-         rewrite inline_cwhile.
-         apply E_WhileTrue with s';[now auto | | ].
-         ++ apply inline_ceval_S with (S n1) ; [now auto | now apply PeanoNat.Nat.max_r_iff].
-         ++ rewrite <- inline_cwhile.
-            apply inline_ceval_S with (S n2); [now auto | reflexivity].
-* destruct IHceval as [n IH].
-  exists (S n).
-  intros.
-  specialize (IH ps0).
-  rewrite inline_ccall.
-  destruct n as [|n].
-  + apply ceval_inf_loop in IH.
-    contradiction IH.
-  + apply IH.
-Qed.
+      ++ apply inline_ceval_S with (S n1); [now auto | reflexivity].
+      ++ rewrite <- inline_cwhile.
+         apply inline_ceval_S with (S n2); [now auto | now apply PeanoNat.Nat.max_l_iff].
+         ** rewrite e.
+            rewrite inline_cwhile.
+            apply E_WhileTrue with s';[now auto | | ].
+      ++ apply inline_ceval_S with (S n1) ; [now auto | now apply PeanoNat.Nat.max_r_iff].
+      ++ rewrite <- inline_cwhile.
+         apply inline_ceval_S with (S n2); [now auto | reflexivity].
+      * destruct IHceval as [n IH].
+        exists (S n).
+        intros.
+        specialize (IH ps0).
+        rewrite inline_ccall.
+        destruct n as [|n].
+      + apply ceval_inf_loop in IH.
+        contradiction IH.
+      + apply IH.
+  Qed.
 
-Lemma ceval_n_inline_ps_S n p s ps  s':
-  ceval p s (k_inliner_ps n ps) s' ->
-  forall m, n <= m -> ceval p s (k_inliner_ps m ps) s'.
-Proof.
-intros.
-apply n_inline_n_inline_ps.
-intros.
-eapply n_ps_inline_n_inline in H.
-apply (inline_ceval_S (S n)).
-* apply H.
-* apply le_n_S.
-  assumption.
-Qed.
+  Lemma ceval_n_inline_ps_S n p s ps  s':
+    ceval p s (k_inliner_ps n ps) s' ->
+    forall m, n <= m -> ceval p s (k_inliner_ps m ps) s'.
+  Proof.
+    intros.
+    apply n_inline_n_inline_ps.
+    intros.
+    eapply n_ps_inline_n_inline in H.
+    apply (inline_ceval_S (S n)).
+    * apply H.
+    * apply le_n_S.
+      assumption.
+  Qed.
 
-(* ceval is inlining insensitive on ps *)
+  (* ceval is inlining insensitive on ps *)
 
-Lemma n_inline_ps_ceval p s ps s' n:
-  ceval p s (k_inliner_ps n ps) s' -> ceval p s ps s'.
-Proof.
-intros.
-apply inline_n_ceval with (S n).
-intros.
-specialize (n_ps_inline_n_inline n p s ps s' H ps0).
-intros.
-apply H0.
-Qed.
+  Lemma n_inline_ps_ceval p s ps s' n:
+    ceval p s (k_inliner_ps n ps) s' -> ceval p s ps s'.
+  Proof.
+    intros.
+    apply inline_n_ceval with (S n).
+    intros.
+    specialize (n_ps_inline_n_inline n p s ps s' H ps0).
+    intros.
+    apply H0.
+  Qed.
 
-Lemma ceval_n_inline_ps p s ps s':
-  ceval p s ps s' -> exists n, ceval p s (k_inliner_ps n ps) s'.
-Proof.
-intros.
-apply ceval_inline_n in H.
-destruct H as [n IH].
-destruct n as [|n].
-* specialize (IH ps).
-  apply ceval_inf_loop in IH.
-  contradiction IH.
-* exists n.
-  apply n_inline_n_inline_ps.
-  apply IH.
-Qed.
+  Lemma ceval_n_inline_ps p s ps s':
+    ceval p s ps s' -> exists n, ceval p s (k_inliner_ps n ps) s'.
+  Proof.
+    intros.
+    apply ceval_inline_n in H.
+    destruct H as [n IH].
+    destruct n as [|n].
+    * specialize (IH ps).
+      apply ceval_inf_loop in IH.
+      contradiction IH.
+    * exists n.
+      apply n_inline_n_inline_ps.
+      apply IH.
+  Qed.
 
-(*Inling "n+1" times on Psi.psi is equivalent to inline p and "n" times Psi.psi*)
+  (*Inling "n+1" times on Psi.psi is equivalent to inline p and "n" times Psi.psi*)
 
-Lemma n_inline_ps_inline  n  f s ps s' :
- ceval (CCall f) s (k_inliner_ps (S n) ps) s' ->
- ceval (inliner (CCall f) ps) s (k_inliner_ps n ps) s'.
-Proof.
-intros.
-apply inline_ceval.
-specialize (n_ps_inline_n_inline (S n) (CCall f) s ps s' H).
-intros.
-apply H0.
-Qed.
+  Lemma n_inline_ps_inline  n  f s ps s' :
+    ceval (CCall f) s (k_inliner_ps (S n) ps) s' ->
+    ceval (inliner (CCall f) ps) s (k_inliner_ps n ps) s'.
+  Proof.
+    intros.
+    apply inline_ceval.
+    specialize (n_ps_inline_n_inline (S n) (CCall f) s ps s' H).
+    intros.
+    apply H0.
+  Qed.
+
+End Inline1.
+
+Module Inline2.
+  Fixpoint k_inliner n c (ps : Psi.psi) :=
+    match n with
+    | 0 => c
+    | S n' => inliner c (fun f => k_inliner n' (ps f) ps)
+    end.
+
+  Definition k_inliner_ps n ps := fun p => k_inliner n (ps p) ps.
+
+  Lemma n_inline_ceval_ceval n c s ps s' :
+    ceval (k_inliner n c ps) s ps s' ->
+    ceval c s ps s'.
+  Proof.
+    generalize dependent ps.
+    generalize dependent c.
+    generalize dependent s.
+    generalize dependent s'.
+    induction n;intros.
+    - apply H.
+    - generalize dependent s.
+      generalize dependent s'.
+      induction c;intros;auto.
+      + inversion H;subst.
+        apply (E_Seq _ s'0).
+        * now auto.
+        * now auto.
+      + inversion H; subst.
+        * apply E_IfTrue; now auto.
+        * apply E_IfFalse; now auto.
+      + remember (k_inliner (S n) (CWhile b c inv var) ps) as original_command eqn:Horig.
+        induction H; inversion Horig;subst.
+        * apply E_WhileFalse; now auto.
+        * eapply E_WhileTrue;[ auto | | ].
+          -- now eauto.
+          -- now auto.
+      + apply IHn in H.
+        apply E_Call.
+        auto.
+  Qed.
+
+  Lemma ceval_n_inline_ceval n c s ps s' :
+    ceval c s ps s' ->
+    ceval (k_inliner n c ps) s ps s'.
+  Proof.
+    generalize dependent ps.
+    generalize dependent c.
+    generalize dependent s.
+    generalize dependent s'.
+    induction n;intros.
+    - apply H.
+    - generalize dependent s.
+      generalize dependent s'.
+      induction c;intros;auto.
+      + inversion H;subst.
+        apply (E_Seq _ s'0).
+        * now auto.
+        * now auto.
+      + inversion H; subst.
+        * apply E_IfTrue; now auto.
+        * apply E_IfFalse; now auto.
+      + remember (CWhile b c inv var) as original_command eqn:Horig.
+        induction H; inversion Horig;subst.
+        * apply E_WhileFalse; now auto.
+        * eapply E_WhileTrue;[ auto | | ].
+          -- now eauto.
+          -- now auto.
+      + simpl.
+        apply IHn.
+        inversion H;subst.
+        auto.
+  Qed.
+
+  Lemma n_inline_ps_ceval_ceval n c s ps s' :
+    ceval c s (k_inliner_ps n ps) s' ->
+    ceval c s ps s'.
+  Proof.
+    intros.
+    remember (k_inliner_ps n ps) as original_command eqn:Horig.
+    induction H.
+    + apply E_Skip.
+    + apply E_Ass. auto.
+    + apply E_Assr. auto.
+    + apply E_Assert.
+    + apply E_IfTrue; now auto.
+    + apply E_IfFalse; now auto.
+    + apply (E_Seq _ s').
+      * now auto.
+      * now auto.
+    + apply E_WhileFalse; now auto.
+    + eapply E_WhileTrue;[ auto | | ].
+      -- now eauto.
+      -- now auto.
+    + specialize (IHceval Horig).
+      rewrite Horig in IHceval.
+      apply n_inline_ceval_ceval in IHceval.
+      apply E_Call.
+      auto.
+  Qed.
+
+End Inline2.
